introduce MS bang type notation and update case studies

theories/case_studies/cooperative_concurrency.v
@@ -27,9 +27,9 @@ From affect.logic Require Import tactics.
 
 (* Make all the definitions opaque so that we do not rely on their definition in the model to show that the programs are well-typed terms. *)
 Opaque sem_typed sem_typed_val ty_le row_le sig_le row_type_sub row_env_sub.
-Opaque sem_ty_void sem_ty_unit sem_ty_bool sem_ty_int sem_ty_string sem_ty_top sem_ty_bang sem_env_bang sem_ty_ref_cpy sem_ty_ref sem_ty_prod sem_ty_sum sem_ty_arr sem_ty_forall sem_ty_row_forall sem_ty_exists sem_ty_rec sem_ty_option sem_ty_list.
-Opaque sem_sig_eff sem_sig_flip_bang.
-Opaque sem_row_nil sem_row_flip_bang sem_row_cons sem_row_rec.
+Opaque sem_ty_bot sem_ty_unit sem_ty_bool sem_ty_int sem_ty_string sem_ty_top sem_ty_mbang env_mbang sem_ty_ref_cpy sem_ty_ref sem_ty_prod sem_ty_sum sem_ty_arr sem_ty_type_forall sem_ty_row_forall sem_ty_exists sem_ty_rec sem_ty_option.
+Opaque sem_sig_eff sem_sig_flip_mbang.
+Opaque sem_row_nil sem_row_flip_mbang sem_row_cons sem_row_rec.
 
 Definition impossible : expr := ((rec: "f" <> := "f" #()) #())%E.
 
@@ -104,22 +104,22 @@ Section typing.
 
   Context `{!heapGS Σ}.
 
-  Definition Queue := Refᶜ (List (() ⊸ ())).
+  Definition Queue := Refᶜ (List (𝟙 ⊸ 𝟙)).
 
-  Definition Status τ := τ + List (τ ⊸ ()).
+  Definition Status τ := τ + List (τ ⊸ 𝟙).
 
   Definition Promise τ := Refᶜ (Status τ).
 
-  Definition await_sig : sem_sig Σ := (∀S: α, Promise ('! α) =[ OS ]=> '! α)%S.
+  Definition await_sig : sem_sig Σ := (∀ₛ α, (Promise (! α)) =[ OS ]=> (! α))%S.
 
   Definition async_sig (θ : sem_row Σ) : sem_sig Σ := 
-    (∀S: α, ( () -{ θ }-∘ '! α ) =[ OS ]=> Promise ('! α))%S. 
+    (∀ₛ α, ( 𝟙 -{ θ }-∘ ! α ) =[ OS ]=> Promise (! α))%S. 
 
   Definition coop_pre (θ : sem_row Σ) : sem_row Σ := 
     (("async", async_sig θ) · ("await", await_sig) · ⟨⟩)%R.
 
   Local Instance await_sig_ne :
-    NonExpansive (λ (α : sem_ty Σ), Promise ('! α)).
+    NonExpansive (λ (α : sem_ty Σ), Promise (! α)).
   Proof.
     rewrite /Promise /Status. intros ?????.
     apply non_dep_fun_dist. by repeat f_equiv.
@@ -127,7 +127,7 @@ Section typing.
 
   Local Instance async_sig_ne θ :
     NonExpansive
-      (λ (α : sem_ty Σ), () -{ θ }-∘ '! α).
+      (λ (α : sem_ty Σ), 𝟙 -{ θ }-∘ ! α).
   Proof.
     intros ?????. apply non_dep_fun_dist.
     do 2 f_equiv; try done. 
@@ -135,9 +135,9 @@ Section typing.
 
   Local Instance async_sig_2_ne : NonExpansive async_sig.
   Proof.
-    intros ????. rewrite /async_sig. apply non_dep_fun_dist.
-    f_equiv. rewrite /tele_app. simpl. intros ?. destruct x0. simpl.
-    by f_equiv.
+    intros ?????. rewrite /async_sig. apply non_dep_fun_dist.
+    f_equiv. rewrite /tele_app. simpl. intros ?. destruct x0. simpl;
+    f_equiv.
   Qed.
 
   Local Instance contractive_coop_pre : Contractive coop_pre.
@@ -166,15 +166,15 @@ Section typing.
     apply sig_eff_os_once; apply _.
   Qed.
 
-  Definition iter_ty τ := (∀R: θ, (τ -{ ¡ θ }-> ()) → List τ -{ ¡ θ }-∘ ())%T.
+  Definition iter_ty τ := (∀R: θ, (τ -{ ¡ θ }-> 𝟙) → List τ -{ ¡ θ }-∘ 𝟙)%T.
   
-  Definition next_ty := (() → ())%T.
+  Definition next_ty := (𝟙 → 𝟙)%T.
 
-  Definition add_ty := ((() ⊸ ()) → ())%T.
+  Definition add_ty := ((𝟙 ⊸ 𝟙) → 𝟙)%T.
 
-  Definition resume_task_ty := (∀T: α, '! α → ('! α ⊸ ()) → ())%T.
+  Definition resume_task_ty := (∀T: α, '! α → ('! α ⊸ 𝟙) → 𝟙)%T.
   
-  Definition runner_ty := (∀T: α, (() -{ coop }-∘ '! α) → '! α)%T.
+  Definition runner_ty := (∀T: α, (𝟙 -{ coop }-∘ '! α) → '! α)%T.
 
   Lemma impossible_typed τ :
     ⊢ ⊨ impossible : ⊥ : τ.
@@ -190,7 +190,7 @@ Section typing.
   Qed.
 
   Lemma async_typed :
-    ⊢ ⊨ᵥ async : (∀T: α, (() -{ coop }-∘ '! α) -{ coop }-> Promise ('! α)).
+    ⊢ ⊨ᵥ async : (∀T: α, (𝟙 -{ coop }-∘ '! α) -{ coop }-> Promise ('! α)).
   Proof.
     rewrite /async. iIntros.
     iApply sem_typed_Tclosure. iIntros (α).
@@ -198,7 +198,7 @@ Section typing.
     iApply sem_typed_sub_row; first iApply row_le_rec_fold.
     rewrite /coop_pre -/coop.
     iApply (sem_typed_perform_os (TT:=[tele _]) [tele_arg (α : sem_ty Σ)] _ "async"
-                                 (tele_app (λ α, () -{ coop }-∘ '! α)) (tele_app (λ α, Promise ('! α)))).
+                                 (tele_app (λ α, 𝟙 -{ coop }-∘ '! α)) (tele_app (λ α, Promise ('! α)))).
     iApply sem_typed_var'.
   Qed.
 
@@ -217,21 +217,21 @@ Section typing.
   Qed.
 
   Lemma yield_typed :
-    ⊢ ⊨ᵥ yield : ( () -{ coop }-> () ).
+    ⊢ ⊨ᵥ yield : ( 𝟙 -{ coop }-> 𝟙 ).
   Proof.
     iIntros. iApply sem_typed_closure; try done. simpl.
-    iApply (sem_typed_app_os (Promise ('! ()))).
+    iApply (sem_typed_app_os (Promise ('! 𝟙))).
     - iApply sem_typed_sub_u2aarr.
       iApply sem_typed_sub_ty; [iApply ty_le_uarr|]; 
         [iApply row_le_refl|iApply ty_le_refl|iApply (ty_le_mbang_elim MS)|].
       iApply sem_typed_sub_nil. simpl. rewrite -/coop.
       set C := (λ α, (Promise ('! α)) -{ coop }-> ('! α)).
-      rewrite -/(C ()). iApply sem_typed_TApp; first solve_copy.
+      rewrite -/(C 𝟙). iApply sem_typed_TApp; first solve_copy.
       iApply sem_typed_val. iApply await_typed.
-    - iApply (sem_typed_app_os (() -{ coop }-∘ '! ())).
+    - iApply (sem_typed_app_os (𝟙 -{ coop }-∘ '! 𝟙)).
       + iApply sem_typed_sub_nil. iApply sem_typed_sub_u2aarr.
-        set C := (λ α, (() -{ coop }-∘ '! α) -{ coop }-> Promise ('! α)).
-        rewrite -/(C ()). iApply sem_typed_TApp; first solve_copy.
+        set C := (λ α, (𝟙 -{ coop }-∘ '! α) -{ coop }-> Promise ('! α)).
+        rewrite -/(C 𝟙). iApply sem_typed_TApp; first solve_copy.
         iApply sem_typed_val. iApply async_typed.
       + iApply sem_typed_sub_nil.
         rewrite - {1} (app_nil_r []).
@@ -247,8 +247,8 @@ Section typing.
     iApply sem_typed_closure; solve_sidecond. simpl.
     rewrite - [[("g", _); ("f", _)]]app_nil_r. 
     iApply sem_typed_afun; solve_sidecond. simpl.
-    set Γ₂ := [("g", τ -{ ¡ σ }-> ());
-               ("f", ((τ -{ ¡ σ }-> ()) → List τ -{ ¡ σ }-∘ ())%T)].
+    set Γ₂ := [("g", τ -{ ¡ σ }-> 𝟙);
+               ("f", ((τ -{ ¡ σ }-> 𝟙) → List τ -{ ¡ σ }-∘ 𝟙)%T)].
     iApply (sem_typed_match_list _ _ _ _ Γ₂); solve_sidecond.
     - iApply sem_typed_var'.
     - do 2 iApply sem_typed_weaken. iApply sem_typed_unit'.
@@ -274,7 +274,7 @@ Section typing.
     iApply sem_typed_closure; solve_sidecond. simpl.
     set q := ("q", Queue). rewrite -(app_nil_r [q]).
     iApply sem_typed_ufun; solve_sidecond. simpl.
-    set f := ("f", () ⊸ ()).
+    set f := ("f", 𝟙 ⊸ 𝟙).
     iApply sem_typed_seq; [|iApply sem_typed_unit].
     iApply sem_typed_replace_cpy_os; [iApply sem_typed_var|].
     iApply sem_typed_cons.
@@ -300,8 +300,8 @@ Section typing.
     - iApply sem_typed_swap_second.
       iApply sem_typed_swap_third.
       iApply sem_typed_swap_second.
-      set x := ("x", () ⊸ ()).
-      set xs := ("xs", List (() ⊸ ())).
+      set x := ("x", 𝟙 ⊸ 𝟙).
+      set xs := ("xs", List (𝟙 ⊸ 𝟙)).
       rewrite -/q.
       iApply sem_typed_seq.
       { iApply sem_typed_replace_cpy_os; iApply sem_typed_var. }
@@ -322,7 +322,7 @@ Section typing.
     rewrite -(app_nil_r [("v", '! α); add]).
     set v := ("v", '! α).
     iApply sem_typed_ufun; solve_sidecond. simpl.
-    set k := ("k", '! α ⊸ ()).
+    set k := ("k", '! α ⊸ 𝟙).
     iApply sem_typed_app_os.
     { iApply sem_typed_sub_u2aarr. iApply sem_typed_var. }
     replace ([k; v; add]) with ([k;v] ++ [add]) by done.
@@ -336,9 +336,9 @@ Section typing.
   Proof.
     iIntros. iApply sem_typed_Tclosure. iIntros (α).
     iApply sem_typed_closure; solve_sidecond. simpl.
-    set main := ("main", () -{ coop }-∘ '! α).
+    set main := ("main", 𝟙 -{ coop }-∘ '! α).
     iApply (sem_typed_let _ _ _ _  [main]); solve_sidecond.
-    { iApply (sem_typed_alloc_cpy (List (() ⊸ ()))). iApply sem_typed_nil. }
+    { iApply (sem_typed_alloc_cpy (List (𝟙 ⊸ 𝟙))). iApply sem_typed_nil. }
     iApply sem_typed_contraction; solve_sidecond.
     set q := ("q", Queue).
     iApply (sem_typed_let _ _ _ _ [q; main]); solve_sidecond.
@@ -363,26 +363,26 @@ Section typing.
     iApply (sem_typed_let _ _ _ _ [main]); solve_sidecond.
     - assert (Hrw : [resume_task;add;next;main] = [resume_task;add;next] ++ [main]) by done.
       rewrite Hrw. clear Hrw. iApply sem_typed_oval.
-      iApply (sem_typed_ufun_poly_rec (λ β, Promise ('! β)) (λ _, ⊥) (λ β, (() -{ coop }-∘ '! β) ⊸ ())); 
+      iApply (sem_typed_ufun_poly_rec (λ β, Promise ('! β)) (λ _, ⊥) (λ β, (𝟙 -{ coop }-∘ '! β) ⊸ 𝟙)); 
         solve_sidecond.
       { iIntros. iApply copy_ty_uarr. }
      simpl. iIntros (β) "/=". 
      set promise := ("promise", Promise ('! β)).
-     set fulfill := ("fulfill", ∀T: β', Promise ('! β') → (() -{ coop }-∘ '! β') ⊸ ()).
+     set fulfill := ("fulfill", ∀T: β', Promise ('! β') → (𝟙 -{ coop }-∘ '! β') ⊸ 𝟙).
      rewrite -(app_nil_r [promise;fulfill;resume_task;add;next]).
      iApply sem_typed_afun; solve_sidecond. simpl.
-     set comp := ("comp", () -{ coop }-∘ '! β)%T.
+     set comp := ("comp", 𝟙 -{ coop }-∘ '! β)%T.
      replace ([comp; promise; fulfill; resume_task; add;next]) with
              ([comp] ++ [promise; fulfill; resume_task; add;next]) by done.
      iApply (sem_typed_handler2 (TT:=[tele _]) OS "async" "await" 
-                    (tele_app (λ α, () -{ coop }-∘ '! α)) 
+                    (tele_app (λ α, 𝟙 -{ coop }-∘ '! α)) 
                     (tele_app (λ α, Promise ('! α))) 
                     (tele_app (λ α, Promise ('! α))) 
                     (tele_app (λ α, '! α))  _ _ _ _ [comp] []); solve_sidecond.
      + iIntros. iApply copy_ty_uarr.
      + iIntros. iApply copy_ty_uarr.
      + iApply row_le_refl.
-     + iApply (sem_typed_app_os () _ ('! β)); [iApply sem_typed_var'|]. 
+     + iApply (sem_typed_app_os 𝟙 _ ('! β)); [iApply sem_typed_var'|]. 
        rewrite -/await_sig -/(async_sig coop) -/coop. 
        iApply sem_typed_sub_env_final; first iApply env_le_cons; first iApply env_le_refl; 
        [iApply ty_le_arr; try iApply ty_le_refl; iApply (row_le_rec_unfold coop_pre)|].
@@ -390,14 +390,14 @@ Section typing.
      + iIntros (β').
        iApply sem_typed_swap_third. iApply sem_typed_weaken.
        iApply sem_typed_swap_fourth. iApply sem_typed_weaken.
-       set x := ("x", () -{ coop }-∘ '! β').
-       set k := ("k", Promise ('!β') ⊸ ()).
+       set x := ("x", 𝟙 -{ coop }-∘ '! β').
+       set k := ("k", Promise ('!β') ⊸ 𝟙).
        rewrite -/x -/k -/fulfill -/add -/next.
        iApply (sem_typed_let (Promise ('! β')) _ _ _ [x;k;fulfill;add;next]); solve_sidecond. 
        { iApply sem_typed_alloc_cpy. iApply sem_typed_right_inj. iApply sem_typed_nil. }
        set new_prom := ("new_prom", Promise ('! β')). 
        iApply (sem_typed_seq _ _ _ _ [new_prom; k; next]).
-       * iApply (sem_typed_app_os (() ⊸ ())%T _ () _ [new_prom; k; add; next]).
+       * iApply (sem_typed_app_os (𝟙 ⊸ 𝟙)%T _ 𝟙 _ [new_prom; k; add; next]).
          { iApply sem_typed_swap_third. iApply sem_typed_sub_u2aarr. iApply sem_typed_var'. }
          iApply sem_typed_swap_fourth. iApply sem_typed_swap_second.
          iApply sem_typed_contraction; solve_sidecond.
@@ -407,7 +407,7 @@ Section typing.
          rewrite Hrw. clear Hrw.
          iApply sem_typed_afun; solve_sidecond. simpl.
          do 2 (iApply sem_typed_swap_second; iApply sem_typed_app_os; [|iApply sem_typed_var]).
-         set C := (λ β, Promise ('! β) → (() -{ coop }-∘ '! β) ⊸ ())%T.
+         set C := (λ β, Promise ('! β) → (𝟙 -{ coop }-∘ '! β) ⊸ 𝟙)%T.
          iApply sem_typed_sub_u2aarr. rewrite -/(C β').
          iApply sem_typed_TApp; first solve_copy. iApply sem_typed_var.
       * simpl.
@@ -415,7 +415,7 @@ Section typing.
         iApply sem_typed_app_os; iApply sem_typed_var'.
      + iIntros (β').
        set x := ("x", Promise ('! β')).
-       set k := ("k", '! β' ⊸ ()).
+       set k := ("k", '! β' ⊸ 𝟙).
        do 4 (iApply sem_typed_swap_third; iApply sem_typed_weaken).
        iApply (sem_typed_match ('! β') _ _  _ _ [x;k;next]); solve_sidecond.
        * iApply sem_typed_replace_cpy_os; first iApply sem_typed_var.
@@ -430,7 +430,7 @@ Section typing.
            iApply sem_typed_left_inj. iApply sem_typed_var. }
          iApply sem_typed_app_os; [iApply sem_typed_var|].
          iApply sem_typed_var.
-       * simpl. set ks := ("ks", List ('! β' ⊸ ())).
+       * simpl. set ks := ("ks", List ('! β' ⊸ 𝟙)).
          iApply (sem_typed_seq (Status ('! β'))).
          ** iApply sem_typed_swap_third. 
             iApply sem_typed_replace_cpy_os; first iApply sem_typed_var.
@@ -451,26 +451,26 @@ Section typing.
       * iApply sem_typed_replace_cpy_os; [|iApply sem_typed_right_inj; iApply sem_typed_nil].
         iApply sem_typed_contraction; solve_sidecond.
         iApply sem_typed_var.
-      * set v := ("v", '! β + (List ('! β ⊸ ()))).
+      * set v := ("v", '! β + (List ('! β ⊸ 𝟙))).
         iApply (sem_typed_match  _ _ _ _ _ [promise; x; resume_task; next]); solve_sidecond;
           [iApply sem_typed_var| |].
         { simpl. do 4 (iApply sem_typed_weaken). iApply impossible_typed. }
         simpl. iApply sem_typed_swap_second. 
         iApply sem_typed_swap_third. iApply sem_typed_contraction; solve_sidecond.
         iApply sem_typed_swap_third. iApply sem_typed_swap_second.
-        set ks := ("ks", List ('! β ⊸ ())).
+        set ks := ("ks", List ('! β ⊸ 𝟙)).
         iApply (sem_typed_seq _ _ _ _ [x; ks; resume_task; next]).
         ** iApply sem_typed_replace_cpy_os; [iApply sem_typed_var|].
            iApply sem_typed_left_inj. iApply sem_typed_var.
-        ** iApply (sem_typed_seq ()).
+        ** iApply (sem_typed_seq 𝟙).
            2: { iApply sem_typed_app_os; [|iApply sem_typed_unit].
                 iApply sem_typed_sub_u2aarr; iApply sem_typed_var. }
            iApply sem_typed_swap_second.
            iApply sem_typed_app_os; [|iApply sem_typed_var].
-           iApply (sem_typed_app_os (('! β ⊸ ()) → ())%T).
+           iApply (sem_typed_app_os (('! β ⊸ 𝟙) → 𝟙)%T).
            2: { iApply sem_typed_app_os; [|iApply sem_typed_var]. 
                 iApply sem_typed_sub_u2aarr.
-                set C := λ β, ('! β → ('! β ⊸ ()) → ())%T. rewrite -/(C β). simpl.
+                set C := λ β, ('! β → ('! β ⊸ 𝟙) → 𝟙)%T. rewrite -/(C β). simpl.
                 iApply sem_typed_TApp; first solve_sidecond. iApply sem_typed_var. }
            iApply sem_typed_sub_u2aarr.
            iApply sem_typed_sub_ty; first iApply ty_le_uarr; 
@@ -479,21 +479,21 @@ Section typing.
            iApply sem_typed_sub_ty; first iApply ty_le_uarr; 
             [iApply row_le_refl|iApply ty_le_refl|iApply ty_le_arr|];
             [iApply (row_le_mfbang_elim OS)|iApply ty_le_refl|iApply ty_le_refl|].
-           set C := (λ (θ : sem_row Σ), (('! β ⊸ ()) -{ ¡ θ }-> ()) → List ('! β ⊸ ()) -{ ¡ θ }-∘ ())%T.
+           set C := (λ (θ : sem_row Σ), (('! β ⊸ 𝟙) -{ ¡ θ }-> 𝟙) → List ('! β ⊸ 𝟙) -{ ¡ θ }-∘ 𝟙)%T.
            rewrite -/(C ⊥).
            iApply sem_typed_RApp; first solve_copy. 
            iApply sem_typed_val. iApply iter_typed.
-  - set fulfill := ("fulfill", ∀T: α, Promise ('! α) → (() -{ coop }-∘ '! α) ⊸ ()).
+  - set fulfill := ("fulfill", ∀T: α, Promise ('! α) → (𝟙 -{ coop }-∘ '! α) ⊸ 𝟙).
     iApply (sem_typed_let _ _ _ _ [fulfill; main]); solve_sidecond.
     { iApply (sem_typed_alloc_cpy (Status ('! α))). 
       iApply sem_typed_right_inj. iApply sem_typed_nil. }
     set pmain := ("pmain", Refᶜ Status ('! α)).
     iApply sem_typed_contraction; solve_sidecond.
     iApply sem_typed_swap_third. iApply sem_typed_swap_second. iApply sem_typed_swap_fourth.
-    iApply (sem_typed_seq ()).
+    iApply (sem_typed_seq 𝟙).
     + do 2 (iApply sem_typed_app_os; [|iApply sem_typed_var]). 
       iApply sem_typed_sub_u2aarr. 
-      set C := (λ α, Promise ('! α) → (() -{ coop }-∘ '! α) ⊸ ())%T.
+      set C := (λ α, Promise ('! α) → (𝟙 -{ coop }-∘ '! α) ⊸ 𝟙)%T.
       rewrite -/(C α).
       iApply sem_typed_TApp. rewrite /C /Promise.
       iApply sem_typed_var.
