theories/case_studies/verboseClose.v
@@ -26,11 +26,11 @@ From affect.logic Require Import tactics.
 
 (* Make all the definitions opaque so that we do not rely on their definition in the model to show that the programs are well-typed terms. *)
 Opaque sem_typed sem_typed_val ty_le row_le sig_le row_type_sub row_env_sub.
-Opaque sem_ty_void sem_ty_unit sem_ty_bool sem_ty_int sem_ty_string sem_ty_top sem_ty_bang sem_env_bang sem_ty_ref_cpy sem_ty_ref sem_ty_prod sem_ty_sum sem_ty_arr sem_ty_forall sem_ty_row_forall sem_ty_exists sem_ty_rec sem_ty_option sem_ty_list.
-Opaque sem_sig_eff sem_sig_flip_bang.
-Opaque sem_row_nil sem_row_flip_bang sem_row_cons sem_row_rec.
+Opaque sem_ty_bot sem_ty_unit sem_ty_bool sem_ty_int sem_ty_string sem_ty_top sem_ty_mbang env_mbang sem_ty_ref_cpy sem_ty_ref sem_ty_prod sem_ty_sum sem_ty_arr sem_ty_type_forall sem_ty_row_forall sem_ty_exists sem_ty_rec sem_ty_option sem_ty_list.
+Opaque sem_sig_eff sem_sig_flip_mbang.
+Opaque sem_row_nil sem_row_flip_mbang sem_row_cons sem_row_rec.
 
-(* The verboseClose example from paper Soundly Hanlding Linearity by Tang et al. *)
+(* The verboseClose example from paper Soundly Handling Linearity by Tang et al. *)
 
 (* Since we do not support files (as in the example) we instead use sub-structurally treated references. *)
 (* the concept is the same: instead of closing a file, we free the reference *)
@@ -43,35 +43,28 @@ Section typing.
 
   Context `{!heapGS Σ}.
 
-  Definition getSig : operation * sem_sig Σ := ("get", ∀S: (_ : sem_ty Σ), () =[OS]=> Str)%S.  
-  Definition printSig : operation * sem_sig Σ := ("print", ∀S: (_ : sem_ty Σ), Str =[MS]=> ())%S.
+  Definition getSig : operation * sem_sig Σ := ("get", ∀ₛ (_ : sem_ty Σ), 𝟙 =[OS]=> Str)%S.  
+  Definition printSig : operation * sem_sig Σ := ("print", ∀ₛ (_ : sem_ty Σ), Str =[MS]=> 𝟙)%S.
   Definition st : sem_row Σ := (getSig · printSig · ⟨⟩)%R.
 
-  Local Instance once_row_get_sig : Once (getSig · ⟨⟩)%R. 
-  Proof.
-    apply row_cons_once; last apply row_nil_once.
-    apply sig_eff_os_once; apply _.
-  Qed.
-
   Lemma verboseFree_typed :
-    ⊢ ⊨ᵥ verboseFree : (Ref 𝔹 -{ st }-> ()).
+    ⊢ ⊨ᵥ verboseFree : (Ref 𝔹 -{ st }-> 𝟙).
   Proof.
-    iIntros. iApply sem_typed_closure; solve_sidecond.
-    simpl. 
-    iApply (sem_typed_let Str _ _ _ [("f", _)]); solve_sidecond.
+    iIntros. iApply sem_typed_closure; first done. simpl. 
+    smart_apply (sem_typed_let Str _ _ _ [("f", _)]).
     - rewrite /st.
       iApply sem_typed_sub_row.
       { iApply row_le_cons_comp; [iApply sig_le_refl|iApply row_le_nil]. }
       iApply sem_typed_frame.
-      iApply (sem_typed_perform_os (TT:=[tele _]) [tele_arg ()%T] ⟨⟩%R "get" 
-                      (tele_app (λ _, ())) (tele_app (λ _, Str))).
+      iApply (sem_typed_perform_os (TT:=[tele _]) [tele_arg 𝟙%T] ⟨⟩%R "get" 
+                      (tele_app (λ _, 𝟙)) (tele_app (λ _, Str))).
       iApply sem_typed_unit'.
     - iApply sem_typed_seq; first iApply sem_typed_sub_nil.
       { iApply sem_typed_frame. iApply sem_typed_free. iApply sem_typed_var. }
       rewrite /st. iApply sem_typed_sub_row; first by iApply row_le_swap_second.
       rewrite -/getSig.
-      iApply (sem_typed_perform_ms (TT:=[tele _]) [tele_arg ()] (getSig · ⟨⟩)%R 
-                      "print" (tele_app (λ _, Str)) (tele_app ((λ _, ())))); solve_copy.
+      iApply (sem_typed_perform_ms (TT:=[tele _]) [tele_arg 𝟙] (getSig · ⟨⟩)%R 
+                      "print" (tele_app (λ _, Str)) (tele_app ((λ _, 𝟙)))).
       iApply sem_typed_var'.
   Qed.
 
