theories/case_studies/app.v
@@ -26,9 +26,9 @@ From affect.logic Require Import tactics.
 
 (* Make all the definitions opaque so that we do not rely on their definition in the model to show that the programs are well-typed terms. *)
 Opaque sem_typed sem_typed_val ty_le row_le sig_le row_type_sub row_env_sub.
-Opaque sem_ty_void sem_ty_unit sem_ty_bool sem_ty_int sem_ty_string sem_ty_top sem_ty_bang sem_env_bang sem_ty_ref_cpy sem_ty_ref sem_ty_prod sem_ty_sum sem_ty_arr sem_ty_forall sem_ty_row_forall sem_ty_exists sem_ty_rec sem_ty_option sem_ty_list.
-Opaque sem_sig_eff sem_sig_flip_bang.
-Opaque sem_row_nil sem_row_flip_bang sem_row_cons sem_row_rec.
+Opaque sem_ty_bot sem_ty_unit sem_ty_bool sem_ty_int sem_ty_string sem_ty_top sem_ty_mbang env_mbang sem_ty_ref_cpy sem_ty_ref sem_ty_prod sem_ty_sum sem_ty_arr sem_ty_type_forall sem_ty_row_forall sem_ty_exists sem_ty_rec sem_ty_option sem_ty_list.
+Opaque sem_sig_eff sem_sig_flip_mbang.
+Opaque sem_row_nil sem_row_flip_mbang sem_row_cons sem_row_rec.
 
 Definition app : val := (λ: "f" "x", "f" "x")%V.
 
@@ -37,17 +37,17 @@ Section typing.
   Context `{!heapGS Σ}.
 
   Definition app_ty : sem_ty Σ := 
-    (∀R: θ, ∀T: α, ∀T: β, (α -{ θ }-∘ β) → α -{ θ }-∘ β)%T.
+    (∀ᵣ θ, ∀ₜ α, ∀ₜ β, (α -{ θ }-∘ β) → α -{ θ }-∘ β)%T.
 
   Lemma app_typed : ⊢ ⊨ᵥ app : app_ty.
   Proof.
     iIntros. rewrite /app /app_ty.
-    iApply sem_typed_Rclosure; solve_sidecond. iIntros (θ).
-    iApply sem_typed_Tclosure; solve_sidecond. iIntros (α).
-    iApply sem_typed_Tclosure; solve_sidecond. iIntros (β).
-    iApply sem_typed_closure; solve_sidecond. simpl.
+    iApply sem_typed_Rclosure. iIntros (θ).
+    iApply sem_typed_Tclosure. iIntros (α).
+    iApply sem_typed_Tclosure. iIntros (β).
+    iApply sem_typed_closure; first done. simpl.
     rewrite - (app_nil_r [("f", _)]).
-    iApply sem_typed_afun; solve_sidecond. simpl.
+    smart_apply sem_typed_afun. simpl.
     iApply sem_typed_app_nil; iApply sem_typed_var'.
   Qed.
 
