theories/case_studies/c.v
@@ -26,9 +26,9 @@ From affect.logic Require Import tactics.
 
 (* Make all the definitions opaque so that we do not rely on their definition in the model to show that the programs are well-typed terms. *)
 Opaque sem_typed sem_typed_val ty_le row_le sig_le row_type_sub row_env_sub.
-Opaque sem_ty_void sem_ty_unit sem_ty_bool sem_ty_int sem_ty_string sem_ty_top sem_ty_bang sem_env_bang sem_ty_ref_cpy sem_ty_ref sem_ty_prod sem_ty_sum sem_ty_arr sem_ty_forall sem_ty_row_forall sem_ty_exists sem_ty_rec sem_ty_option sem_ty_list.
-Opaque sem_sig_eff sem_sig_flip_bang.
-Opaque sem_row_nil sem_row_flip_bang sem_row_cons sem_row_rec.
+Opaque sem_ty_bot sem_ty_unit sem_ty_bool sem_ty_int sem_ty_string sem_ty_top sem_ty_mbang env_mbang sem_ty_ref_cpy sem_ty_ref sem_ty_prod sem_ty_sum sem_ty_arr sem_ty_type_forall sem_ty_row_forall sem_ty_exists sem_ty_rec sem_ty_option sem_ty_list.
+Opaque sem_sig_eff sem_sig_flip_mbang.
+Opaque sem_row_nil sem_row_flip_mbang sem_row_cons sem_row_rec.
 
 Definition C : val := (λ: "x" "y" "z", ("x" "z") "y")%V.
 
@@ -37,28 +37,28 @@ Section typing.
   Context `{!heapGS Σ}.
 
   Definition C_os_ty : sem_ty Σ := 
-    (∀R: θ, ∀T: α, ∀T: β, ∀T: γ,  (β -{ ¡ θ }-∘ (α -{ ¡ θ }-∘ γ)) → α ⊸ β -{ ¡ θ }-∘ γ)%T.
+    (∀ᵣ θ, ∀ₜ α, ∀ₜ β, ∀ₜ γ,  (β -{ ¡ θ }-∘ (α -{ ¡ θ }-∘ γ)) → α ⊸ β -{ ¡ θ }-∘ γ)%T.
 
   Definition C_ms_ty : sem_ty Σ := 
-    (∀R: θ, ∀T: α, ∀T: β, ∀T: γ,  (β -{ θ }-∘ ('! α -{ θ }-∘ γ)) → ('! α) ⊸ β -{ θ }-∘ γ)%T.
+    (∀ᵣ θ, ∀ₜ α, ∀ₜ β, ∀ₜ γ,  (β -{ θ }-∘ (! α -{ θ }-∘ γ)) → (! α) ⊸ β -{ θ }-∘ γ)%T.
 
   Definition C_gen_ty : sem_ty Σ := 
-    (∀M: ν, ∀R: θ, ∀T: α, ∀T: β, ∀T: γ, (β -{ ¡_[ ν ] θ }-∘ ('!_[ν] α -{ ¡_[ ν ] θ }-∘ γ)) → ('!_[ ν ] α) ⊸ β -{ ¡_[ ν ] θ }-∘ γ)%T.
+    (∀ₘ ν, ∀ᵣ θ, ∀ₜ α, ∀ₜ β, ∀ₜ γ, (β -{ ¡[ν] θ }-∘ (![ν] α -{ ¡[ν] θ }-∘ γ)) → (![ν] α) ⊸ β -{ ¡[ν] θ }-∘ γ)%T.
 
   Lemma C_os_typed : ⊢ ⊨ᵥ C : C_os_ty.
   Proof.
     iIntros. rewrite /C /C_os_ty.
-    iApply sem_typed_Rclosure; solve_sidecond. iIntros (θ).
-    iApply sem_typed_Tclosure; solve_sidecond. iIntros (α).
-    iApply sem_typed_Tclosure; solve_sidecond. iIntros (β).
-    iApply sem_typed_Tclosure; solve_sidecond. iIntros (γ).
-    iApply sem_typed_closure; solve_sidecond. simpl.
+    iApply sem_typed_Rclosure; iIntros (θ).
+    iApply sem_typed_Tclosure; iIntros (α).
+    iApply sem_typed_Tclosure; iIntros (β).
+    iApply sem_typed_Tclosure; iIntros (γ).
+    iApply sem_typed_closure; first done. simpl.
     rewrite - (app_nil_r [("x", _)]).
-    iApply sem_typed_afun; solve_sidecond. simpl.
+    smart_apply sem_typed_afun. simpl.
     rewrite - (app_nil_r [("y", _); ("x", _)]).
-    iApply sem_typed_afun; solve_sidecond. simpl.
+    smart_apply sem_typed_afun. simpl.
     iApply sem_typed_swap_second.
-    iApply (sem_typed_app_os α (¡θ)%R); solve_sidecond.
+    iApply (sem_typed_app_os α (¡θ)%R).
     { iApply sem_typed_app_os; iApply sem_typed_var'. }
     iApply sem_typed_var'.
   Qed.
@@ -66,17 +66,17 @@ Section typing.
   Lemma C_ms_typed : ⊢ ⊨ᵥ C : C_ms_ty.
   Proof.
     iIntros. rewrite /C /C_ms_ty.
-    iApply sem_typed_Rclosure; solve_sidecond. iIntros (θ).
-    iApply sem_typed_Tclosure; solve_sidecond. iIntros (α).
-    iApply sem_typed_Tclosure; solve_sidecond. iIntros (β).
-    iApply sem_typed_Tclosure; solve_sidecond. iIntros (γ).
-    iApply sem_typed_closure; solve_sidecond. simpl.
+    iApply sem_typed_Rclosure; iIntros (θ).
+    iApply sem_typed_Tclosure; iIntros (α).
+    iApply sem_typed_Tclosure; iIntros (β).
+    iApply sem_typed_Tclosure; iIntros (γ).
+    iApply sem_typed_closure; first done. simpl.
     rewrite - (app_nil_r [("x", _)]).
-    iApply sem_typed_afun; solve_sidecond. simpl.
+    smart_apply sem_typed_afun. simpl.
     rewrite - (app_nil_r [("y", _); ("x", _)]).
-    iApply sem_typed_afun; solve_sidecond. simpl.
+    smart_apply sem_typed_afun. simpl.
     iApply sem_typed_swap_second.
-    iApply (sem_typed_app_ms ('! α)); solve_sidecond.
+    iApply (sem_typed_app_ms (! α)).
     { iApply sem_typed_app_nil; iApply sem_typed_var'. }
     iApply sem_typed_var'.
   Qed.
@@ -84,26 +84,22 @@ Section typing.
   Lemma C_gen_typed : ⊢ ⊨ᵥ C : C_gen_ty.
   Proof.
     iIntros. rewrite /C_gen_ty /C.
-    iApply sem_typed_Mclosure; solve_sidecond. iIntros (ν).
-    iApply sem_typed_Rclosure; solve_sidecond. iIntros (θ).
-    iApply sem_typed_Tclosure; solve_sidecond. iIntros (α).
-    iApply sem_typed_Tclosure; solve_sidecond. iIntros (β).
-    iApply sem_typed_Tclosure; solve_sidecond. iIntros (γ).
-    iApply sem_typed_closure; solve_sidecond. simpl.
+    iApply sem_typed_Mclosure. iIntros (ν).
+    iApply sem_typed_Rclosure. iIntros (θ).
+    iApply sem_typed_Tclosure. iIntros (α).
+    iApply sem_typed_Tclosure. iIntros (β).
+    iApply sem_typed_Tclosure. iIntros (γ).
+    iApply sem_typed_closure; first done. simpl.
     rewrite - (app_nil_r [("x", _)]).
-    iApply sem_typed_afun; solve_sidecond. simpl.
+    smart_apply sem_typed_afun. simpl.
     rewrite - (app_nil_r [("y", _); ("x", _)]).
-    iApply sem_typed_afun; solve_sidecond. simpl.
+    smart_apply sem_typed_afun. simpl.
     rewrite - (app_nil_r [("y", _); ("x", _)]).
-    iApply (sem_typed_app_gen ('!_[ ν ] α) (¡_[ ν ] θ)%R (¡_[ ν ] θ)%R (¡_[ ν ] θ)%R).
+    iApply (sem_typed_app_gen (![ν] α) (¡[ν] θ)%R (¡[ν] θ)%R (¡[ν] θ)%R).
     - iApply row_le_refl.
-    - iApply row_type_sub_mfbang_mbang.
-    - iApply row_env_sub_copy; solve_copy.
     - iApply row_le_refl.
-    - iApply (sem_typed_app_gen β (¡ ⟨⟩)%R (¡_[ ν ] θ)%R (¡_[ ν ] θ)%R).
-      + iApply row_le_trans; [iApply (row_le_mfbang_elim OS)|iApply row_le_nil].
-      + iApply row_type_sub_fbang.
-      + iApply row_env_sub_copy; solve_copy.
+    - iApply (sem_typed_app_gen β (¡ ⟨⟩)%R (¡[ν] θ)%R (¡[ν] θ)%R).
+      + iApply row_le_trans; [iApply (row_le_mfbang_elim_nil OS)|iApply row_le_nil].
       + iApply row_le_refl.
       + iApply sem_typed_var'.
       + iApply sem_typed_var'.
