theories/case_studies/hid.v
@@ -25,9 +25,9 @@ From affect.logic Require Import tactics.
 
 (* Make all the definitions opaque so that we do not rely on their definition in the model to show that the programs are well-typed terms. *)
 Opaque sem_typed sem_typed_val ty_le row_le sig_le row_type_sub row_env_sub.
-Opaque sem_ty_void sem_ty_unit sem_ty_bool sem_ty_int sem_ty_string sem_ty_top sem_ty_bang sem_env_bang sem_ty_ref_cpy sem_ty_ref sem_ty_prod sem_ty_sum sem_ty_arr sem_ty_forall sem_ty_row_forall sem_ty_exists sem_ty_rec sem_ty_option sem_ty_list.
-Opaque sem_sig_eff sem_sig_flip_bang.
-Opaque sem_row_nil sem_row_flip_bang sem_row_cons sem_row_rec.
+Opaque sem_ty_bot sem_ty_unit sem_ty_bool sem_ty_int sem_ty_string sem_ty_top sem_ty_mbang env_mbang sem_ty_ref_cpy sem_ty_ref sem_ty_prod sem_ty_sum sem_ty_arr sem_ty_type_forall sem_ty_row_forall sem_ty_exists sem_ty_rec sem_ty_option sem_ty_list.
+Opaque sem_sig_eff sem_sig_flip_mbang.
+Opaque sem_row_nil sem_row_flip_mbang sem_row_cons sem_row_rec.
 
 Definition hid : val := (λ: "f" "x", "f" #();; "x")%V.
 
@@ -36,7 +36,7 @@ Section typing.
   Context `{!heapGS Σ}.
 
   Definition hid_ty : sem_ty Σ := 
-    (∀M: ν, ∀R: θ, ∀T: α, (() -{ ¡_[ ν ] θ }-∘ ()) → '!_[ ν ] α -{ ¡_[ ν ] θ }-∘ α)%T.
+    (∀ₘ ν, ∀ᵣ θ, ∀ₜ α, (𝟙 -{ ¡[ν] θ }-∘ 𝟙) → ![ν] α -{ ¡[ν] θ }-∘ α)%T.
 
   Lemma hid_typed : ⊢ ⊨ᵥ hid : hid_ty.
   Proof.
@@ -48,12 +48,9 @@ Section typing.
     rewrite - (app_nil_r [("f", _)]).
     iApply sem_typed_afun; solve_sidecond. simpl.
     iApply sem_typed_swap_second.
-    iApply (sem_typed_seq () (¡_[ ν ] θ)%R _ _ [("x", ('!_[ν] α)%T)]).
-    - iApply (sem_typed_app_gen () (¡ ⟨⟩)%R (¡_[ν] θ)%R (¡_[ν] θ)%R).
-      + iApply row_le_trans; [iApply (row_le_mfbang_elim OS)|iApply row_le_nil].
-      + iApply row_type_sub_fbang.
-      + iApply row_env_sub_cons; first iApply row_env_sub_copy; solve_copy.  
-        iApply row_type_sub_mfbang_mbang.
+    iApply (sem_typed_seq 𝟙 (¡[ν] θ)%R _ _ [("x", (![ν] α)%T)]).
+    - iApply (sem_typed_app_gen 𝟙 (¡ ⟨⟩)%R (¡[ν] θ)%R (¡[ν] θ)%R).
+      + iApply row_le_trans; [iApply (row_le_mfbang_elim_nil)|iApply row_le_nil].
       + iApply row_le_refl. 
       + iApply sem_typed_var'.
       + iApply sem_typed_unit'.
