theories/case_studies/tossCoin.v
@@ -25,12 +25,11 @@ From affect.logic Require Import tactics.
 
 (* Make all the definitions opaque so that we do not rely on their definition in the model to show that the programs are well-typed terms. *)
 Opaque sem_typed sem_typed_val ty_le row_le sig_le row_type_sub row_env_sub.
-Opaque sem_ty_void sem_ty_unit sem_ty_bool sem_ty_int sem_ty_string sem_ty_top sem_ty_bang sem_env_bang sem_ty_ref_cpy sem_ty_ref sem_ty_prod sem_ty_sum sem_ty_arr sem_ty_forall sem_ty_row_forall sem_ty_exists sem_ty_rec sem_ty_option sem_ty_list.
-Opaque sem_sig_eff sem_sig_flip_bang.
-Opaque sem_row_nil sem_row_flip_bang sem_row_cons sem_row_rec.
+Opaque sem_ty_bot sem_ty_unit sem_ty_bool sem_ty_int sem_ty_string sem_ty_top sem_ty_mbang env_mbang sem_ty_ref_cpy sem_ty_ref sem_ty_prod sem_ty_sum sem_ty_arr sem_ty_type_forall sem_ty_row_forall sem_ty_exists sem_ty_rec sem_ty_option sem_ty_list.
+Opaque sem_sig_eff sem_sig_flip_mbang.
+Opaque sem_row_nil sem_row_flip_mbang sem_row_cons sem_row_rec.
 
 (* The tossCoin example from paper Soundly Hanlding Linearity by Tang et al. *)
-
 Definition tossCoin : val := 
   (λ: "g", let: "b" := "g" #() in 
            if: "b" then #(LitStr "heads") else #(LitStr "tails"))%V.
@@ -40,7 +39,7 @@ Section typing.
   Context `{!heapGS Σ}.
 
   Definition tossCoin_ty : sem_ty Σ := 
-    (∀R: θ, (() -{ θ }-> 𝔹) -{ θ }-> Str)%T.
+    (∀ᵣ θ, (𝟙 -{ θ }-> 𝔹) -{ θ }-> Str)%T.
 
   Lemma tossCoin_typed : ⊢ ⊨ᵥ tossCoin : tossCoin_ty.
   Proof.
@@ -48,7 +47,7 @@ Section typing.
     iApply sem_typed_Rclosure; solve_sidecond. iIntros (θ).
     iApply sem_typed_closure; solve_sidecond. simpl.
     iApply (sem_typed_let 𝔹 θ Str _ []); solve_sidecond.
-    - iApply (sem_typed_app_ms ()); solve_sidecond.
+    - iApply (sem_typed_app_ms 𝟙); solve_sidecond.
       { iApply sem_typed_sub_ty; first iApply ty_le_u2aarr.
         iApply sem_typed_var'. }
       iApply sem_typed_unit'.
