theories/logic/sem_env.v
@@ -4,10 +4,6 @@ From iris.program_logic Require Import weakestpre.
 
 From stdpp Require Import base gmap.
 
-(* Hazel Reasoning *)
-From hazel.program_logic Require Import weakest_precondition 
-                                        state_reasoning.
-
 (* Local imports *)
 From affect.lib Require Import base.
 From affect.lang Require Import affect.
